theories/Stacks.v
@@ -1,0 +1,117 @@
+(** * LogRel.Stacks: definition of stacks, representing evaluation contexts. *)
+From Coq Require Import List.
+From LogRel.AutoSubst Require Import core unscoped Ast Extra.
+From LogRel Require Import Utils BasicAst NormalForms.
+
+Lemma rev_rec :
+forall [A : Type] (P : list A -> Type),
+P nil ->
+(forall (x : A) (l : list A), P l -> P (l ++ x :: nil)) ->
+forall l : list A, P l.
+Proof.
+  intros.
+  rewrite <- rev_involutive.
+  induction (rev l) ; eauto.
+Qed.
+
+Variant ty_entry : term -> Type :=
+  | eSort s : ty_entry (tSort s)
+  | eProd A B : ty_entry (tProd A B)
+  | eNat : ty_entry tNat
+  | eEmpty : ty_entry tEmpty
+  | eSig A B : ty_entry (tSig A B).
+
+Variant nat_entry : term -> Type :=
+  | eZero : nat_entry tZero
+  | eSucc t : nat_entry (tSucc t).
+
+Variant dest_entry : Type :=
+  | eEmptyElim (P : term)
+  | eNatElim (P : term) (hs hz : term)
+  | eApp (u : term)
+  | eFst
+  | eSnd.
+
+Definition zip1 (t : term) (e : dest_entry) : term :=
+  match e with
+    | eEmptyElim P => (tEmptyElim P t)
+    | eNatElim P hs hz => (tNatElim P hs hz t) 
+    | eApp u => (tApp t u)
+    | eFst => tFst t
+    | eSnd => tSnd t
+  end.
+
+Definition stack := list dest_entry.
+
+Fixpoint zip t (π : stack) :=
+  match π with
+  | nil => t
+  | cons s π => zip (zip1 t s) π
+  end.
+
+Section NfEntries.
+
+Lemma zip_app t (π π' : stack) :
+  zip t (π ++ π')%list = zip (zip t π) π'.
+Proof.
+  induction π in t |- * ; cbn.
+  - reflexivity.
+  - apply IHπ.
+Qed.
+
+Lemma zip_whne n π :
+  whne n -> whne (zip n π).
+Proof.
+  intros Hne.
+  induction π as [|[]] in n, Hne |- * ; cbn.
+  1: eassumption.
+  all: eapply IHπ ; now econstructor.
+Qed.
+
+Lemma stack_whne t :
+  whne t <~> ∑ (s : stack) (n : nat), t = zip (tRel n) s.
+Proof.
+  split.
+  - induction 1.
+    1:
+    { exists nil.
+      eexists.
+      reflexivity.
+    }
+    all: destruct IHwhne as (?&?&?) ; subst.
+    1: eexists (_ ++ (eApp _ :: nil))%list.
+    2: eexists (_ ++ (eNatElim _ _ _ :: nil))%list.
+    3: eexists (_ ++ (eEmptyElim _ :: nil))%list.
+    4: eexists (_ ++ (eFst :: nil))%list.
+    5: eexists (_ ++ (eSnd :: nil))%list.
+    all: eexists.
+    all: rewrite zip_app ; cbn.
+    all: reflexivity.
+  - intros (π&n&->).
+    apply zip_whne.
+    now constructor.
+Qed.
+
+Lemma isType_entry t :
+  ty_entry t <~> (isType t × isCanonical t).
+Proof.
+  split.
+  - intros [].
+    all: split ; now constructor.
+  - intros [[] i] ; cycle -1.
+    1: now edestruct can_whne.
+    all: now constructor.
+Qed.
+
+Lemma isNat_entry t :
+  nat_entry t <~> (isNat t × isCanonical t).
+Proof.
+  split.
+  - intros [].
+    all: split ; now constructor.
+  - intros [[] i] ; cycle -1.
+    1: now edestruct can_whne.
+    all: now constructor.
+Qed.
+
+End NfEntries.
